Calculus/Chapter5/Problem_5_13.v
@@ -1,8 +1,7 @@
 From Calculus.Chapter5 Require Import Prelude.
 
 Lemma lemma_5_13 : ∀ f g h a L,
-  (∀ x, f x ≤ g x ≤ h x) →
-    ⟦ lim a ⟧ f = L → ⟦ lim a ⟧ h = L → ⟦ lim a ⟧ g = L.
+  (∀ x, f x ≤ g x ≤ h x) → ⟦ lim a ⟧ f = L → ⟦ lim a ⟧ h = L → ⟦ lim a ⟧ g = L.
 Proof.
   intros f g h a L H1 H2 H3 ε H4.
   specialize (H2 ε H4) as [δ1 [H5 H6]].
