Calculus/Chapter5/Problem_5_18.v
@@ -1,7 +1,13 @@
 From Calculus.Chapter5 Require Import Prelude.
 
 Lemma lemma_5_18 : ∀ f a l,
-  ⟦ lim a ⟧ f = l →
-  ∃ δ M, δ > 0 /\ (∀ x, 0 < |x - a| < δ → |f x| < M).
+  ⟦ lim a ⟧ f = l → ∃ δ M, δ > 0 /\ (∀ x, 0 < |x - a| < δ → |f x| < M).
 Proof.
-Admitted.
+  intros f a l H1.
+  specialize (H1 1 ltac:(solve_R)) as [δ [H2 H3]].
+  exists δ, (|l| + 1). 
+  split; auto.
+  intros x H4.
+  specialize (H3 x H4).
+  solve_R.
+Qed.
