Calculus/Chapter5/Problem_5_19.v
@@ -1,7 +1,7 @@
 From Calculus.Chapter5 Require Import Prelude.
 
-Lemma lemma_5_19 : ∀ (f : R → R) (a : R),
-  (∀ x, irrational x → f x = 0) →
-  (∀ x, rational x → f x = 1) →
-  ∀ L, ¬ (⟦ lim a ⟧ f = L).
-Proof. Admitted.
+Lemma lemma_5_19 : ∀ f a,
+  (∀ x, irrational x → f x = 0) → (∀ x, rational x → f x = 1) → ∀ L, ¬ (⟦ lim a ⟧ f = L).
+Proof.
+
+Admitted.
